Fibonacci reification

teaching/eutypes2018/sol/FibonacciReify.fst
@@ -53,27 +53,37 @@ effect St (a:Type) = STATE a (fun _ p -> forall x s1 . p (x,s1))
 let rec fibonacci_tot (n:nat) : Tot nat 
   = if n <= 1 then 1 else fibonacci_tot (n - 1) + fibonacci_tot (n - 2)
 
-let rec fibonacci (i:pos) : St unit = 
-  if i > 2 then (let temp = STATE?.get_right () in
-                 STATE?.put_right (STATE?.get_left () + STATE?.get_right ()); 
-                 STATE?.put_left temp;
-                 fibonacci (i - 1))
+let rec lemma_fibonacci_tot (n:pos)
+  : Lemma (fibonacci_tot (n + 1) = fibonacci_tot (n - 1) + fibonacci_tot n)
+  = ()
 
-(* let rec fibonacci (i:pos) (n:nat{n >= i}) : St unit (decreases (n - i)) = 
+let rec fibonacci (i:pos) (n:nat{n >= i}) : St unit (decreases (n - i)) = 
   if i < n then (let temp = STATE?.get_right () in
                  STATE?.put_right (STATE?.get_left () + STATE?.get_right ()); 
                  STATE?.put_left temp;
-                 fibonacci (i+1) n) *)
+                 fibonacci (i+1) n)
 
-let lemma_fibonacci_two (i:pos) (m n:int)
-  : Lemma (requires (i <= 2))
-          (ensures  (let (_,(s,s')) = reify (fibonacci i) (m,n) in 
-                     s = m /\ s' = n))
+#set-options "--z3rlimit 32"
+
+let lemma_fibonacci_step (i:pos) (n:nat{n >= i + 1})
+  : Lemma (requires (True))
+          (ensures  (reify (fibonacci (i+1) n) (fibonacci_tot i,fibonacci_tot (i+1)) ==
+                     reify (fibonacci i n) (fibonacci_tot (i-1),fibonacci_tot i)))
+          (decreases (n-i))
   = ()
 
-let rec lemma_fibonacci (i:pos) (m:pos)
+let rec lemma_fibonacci_inv (i:pos) (n:nat{n >= i})
   : Lemma (requires True)
-          (ensures (let (_,(s,s')) = reify (fibonacci i) (fibonacci_tot m, fibonacci_tot (m + 1)) in 
-                    s  = fibonacci_tot (i + m - 2) /\ 
-                    s' = fibonacci_tot (i + m - 1)))
-= admit ()
+          (ensures (let (_,(s,s')) = reify (fibonacci i n) (fibonacci_tot (i - 1), fibonacci_tot i) in 
+                    s  = fibonacci_tot (n - 1) /\ 
+                    s' = fibonacci_tot n))
+          (decreases (n - i))
+  = if i >= n then ()
+              else (lemma_fibonacci_inv (i+1) n; 
+                    lemma_fibonacci_step i n)
+
+let rec lemma_fibonacci (n:pos)
+  : Lemma ((let (_,(s,s')) = reify (fibonacci 1 n) (1, 1) in 
+            s  = fibonacci_tot (n - 1) /\ 
+            s' = fibonacci_tot n))
+  = lemma_fibonacci_inv 1 n
